WIP: added threeway simulations from the SECOMP github + worked more on the RSC_DC_MD proof.

Common/SmallstepUB.v
@@ -73,3 +73,265 @@ Section SEMANTICS.
       step L2 ge s t s'.
 
 End SEMANTICS.
+
+
+
+
+(** * The following code was taken from the following git:
+    https://github.com/secure-compilation/SECOMP
+    file common/Smallstep.v
+*)
+
+(** * Three-way simulations used in recomposition. *)
+
+
+Require Import Coq.micromega.Lia.
+
+Record tsim_properties (L1 L2 L3: semantics)
+                       {single_L1: single_events L1} {single_L2: single_events L2} {single_L3: single_events L3}
+                       (* (index: Type) *)
+                       (* (order: index -> index -> Prop) *)
+                       (match_states: (* index ->  *)state L1 -> state L2 -> state L3 -> Prop) : Prop := {
+    (* tsim_order_wf: well_founded order; *)
+    tsim_match_initial_states:
+      forall s1 s2, initial_state L1 s1 ->
+               initial_state L2 s2 ->
+      exists s3, initial_state L3 s3 /\ match_states s1 s2 s3;
+    (* tsim_match_final_states: *)
+    (*   forall i s1 s2 s3 r, *)
+    (*   match_states i s1 s2 s3 -> final_state L1 s1 r -> final_state L2 s2 r -> final_state L3 s3 r; *)
+    tsim_simulation_simultaneous:
+    forall s1 e s1',
+      Step L1 s1 (e :: nil) s1' ->
+    forall s2 s2', Step L2 s2 (e :: nil) s2' ->
+      forall s3, match_states s1 s2 s3 ->
+      exists s3',
+         (Plus L3 s3 (e :: nil) s3')
+         /\ match_states s1' s2' s3';
+    tsim_simulation1:
+      forall s1 s1', Step L1 s1 E0 s1' ->
+      forall s2 s3, match_states s1 s2 s3 ->
+      exists s3',
+         Star L3 s3 E0 s3'
+      /\ match_states s1' s2 s3';
+    tsim_simulation2:
+      forall s2 s2', Step L2 s2 E0 s2' ->
+      forall s1 s3, match_states s1 s2 s3 ->
+       exists s3',
+         Star L3 s3 E0 s3'
+      /\ match_states s1 s2' s3' }
+  .
+
+Arguments tsim_properties: clear implicits.
+
+Inductive threeway_simulation (L1 L2 L3: semantics)
+  {single_L1: single_events L1} {single_L2: single_events L2} {single_L3: single_events L3} : Prop :=
+  Threeway_simulation (match_states: state L1 -> state L2 -> state L3 -> Prop)
+                      (props: tsim_properties L1 L2 L3 single_L1 single_L2 single_L3
+                                match_states).
+
+Arguments Threeway_simulation {L1 L2 L3 single_L1 single_L2 single_L3 }
+  match_states props.
+(** ** Three-way simulation of transition sequences *)
+
+Section TSIMULATION_SEQUENCES.
+
+Context L1 L2 L3
+  {single_L1: single_events L1} {single_L2: single_events L2} {single_L3: single_events L3}
+   match_states
+  (S: tsim_properties L1 L2 L3 single_L1 single_L2 single_L3 match_states).
+
+Lemma tsimulation_star:
+  forall s1 t s1',
+    Star L1 s1 t s1' ->
+  forall s2 s2',
+    Star L2 s2 t s2' ->
+  forall s3, match_states s1 s2 s3 ->
+  exists s3', Star L3 s3 t s3' /\ match_states s1' s2' s3'.
+Proof.
+  induction 1; intros until s2'.
+  - intros H; remember E0 as t; revert H Heqt.
+    induction 1; intros.
+    + exists s3; split; auto. apply star_refl.
+    + subst t.
+      assert (t1 = E0) by now destruct t1. subst t1.
+      assert (t2 = E0) by now destruct t2. subst t2.
+      exploit tsim_simulation2; eauto.
+      intros [s3' [A B]].
+      exploit IHstar; eauto.
+      intros [s3'' [C D]].
+      eexists; split; auto. eapply star_trans; eauto. eauto.
+  - induction 1; intros.
+    + assert (t1 = E0) by now destruct t1. subst t1.
+      assert (t2 = E0) by now destruct t2. subst t2.
+      exploit tsim_simulation1; eauto.
+      intros [s3' [A B]].
+      exploit IHstar; eauto. eapply star_refl.
+      intros [s3'' [C D]].
+      exists s3''; split; auto. eapply star_trans; eauto.
+    + destruct t1, t0; eauto.
+      * simpl in *; subst t2; subst t3.
+        exploit tsim_simulation1; eauto.
+        intros [s3' [A B]].
+        pose proof (tsim_simulation2 S _ _ H2 _ _ B).
+        destruct H1 as [s3'' [D E]].
+        specialize (IHstar _ _ H3 _ E) as [s3''' [F G]].
+        exists s3'''; split; auto. eapply star_trans; eauto. eapply star_trans; eauto.
+        traceEq.
+      * assert (t0 = nil) by now apply single_L2 in H2; destruct t0; eauto; simpl in H2; lia.
+        subst t0; simpl in *; subst t2; subst t.
+        exploit tsim_simulation1; eauto.
+        intros [s3' [A B]].
+        exploit IHstar. eapply star_step; eauto. eauto.
+        intros [s3'' [C D]].
+        exists s3''; split; auto. eapply star_trans; eauto.
+      * assert (t1 = nil) by now apply single_L1 in H; destruct t1; eauto; simpl in H; lia.
+        subst t1; simpl in *; subst t3; subst t.
+        exploit tsim_simulation2; eauto.
+        intros [s3' [A B]].
+        exploit IHstar0. reflexivity. eauto.
+        intros [s3'' [C D]].
+        exists s3''; split; auto. eapply star_trans; eauto.
+      * assert (t1 = nil) by now apply single_L1 in H; destruct t1; eauto; simpl in H; lia.
+        assert (t0 = nil) by now apply single_L2 in H2; destruct t0; eauto; simpl in H2; lia.
+        subst. simpl in H4. inv H4.
+        exploit tsim_simulation_simultaneous; eauto.
+        intros [s3' [A B]].
+        exploit IHstar; eauto.
+        intros [s3'' [C D]].
+        exists s3''; split; auto. eapply star_trans; eauto. apply plus_star; eauto.
+Qed.
+
+
+End TSIMULATION_SEQUENCES.
+
+Section THREEWAY_SIMU_DIAGRAM.
+
+Variable L1: semantics.
+Variable L2: semantics.
+Variable L3: semantics.
+Context {single_L1: single_events L1}
+  {single_L2: single_events L2}
+  {single_L3: single_events L3}.
+
+Variable metadata: Type.
+
+
+Variable common_equivalence: metadata -> state L1 -> state L2 -> state L3 -> Prop.
+Variable strong_equivalence1: metadata -> state L1 -> state L3 -> Prop.
+Variable strong_equivalence2: metadata -> state L2 -> state L3 -> Prop.
+Variable weak_equivalence1: metadata -> state L1 -> state L3 -> Prop.
+Variable weak_equivalence2: metadata -> state L2 -> state L3 -> Prop.
+
+Variant match_states: metadata -> state L1 -> state L2 -> state L3 -> Prop :=
+  | match_states_left: forall M s1 s2 s3,
+      common_equivalence M s1 s2 s3 ->
+      strong_equivalence1 M s1 s3 ->
+      weak_equivalence2 M s2 s3 ->
+      match_states M s1 s2 s3
+  | match_states_right: forall M s1 s2 s3,
+      common_equivalence M s1 s2 s3 ->
+      weak_equivalence1 M s1 s3 ->
+      strong_equivalence2 M s2 s3 ->
+      match_states M s1 s2 s3.
+
+Hypothesis match_initial_states:
+  forall s1, initial_state L1 s1 ->
+  forall s2, initial_state L2 s2 ->
+  exists s3 M, initial_state L3 s3 /\ match_states M s1 s2 s3.
+
+(* Variable order: (metadata * state L1 * state L2) -> (metadata * state L1 * state L2) -> Prop. *)
+(* Hypothesis order_wf: well_founded order. *)
+
+
+(* The strongly-related states take a silent step at the same time *)
+Hypothesis step_silent_strong1:
+  forall s1 s1', Step L1 s1 E0 s1' ->
+  forall s2 s3 M, strong_equivalence1 M s1 s3 ->
+           weak_equivalence2 M s2 s3 ->
+      common_equivalence M s1 s2 s3 ->
+  exists s3' M', Plus L3 s3 E0 s3' /\ (* Using Plus to ensure the strongly related states take a step *)
+           strong_equivalence1 M' s1' s3' /\
+           weak_equivalence2 M' s2 s3' /\
+              common_equivalence M' s1' s2 s3'.
+
+Hypothesis step_silent_strong2:
+  forall s2 s2', Step L2 s2 E0 s2' ->
+  forall s1 s3 M, strong_equivalence2 M s2 s3 ->
+           weak_equivalence1 M s1 s3 ->
+      common_equivalence M s1 s2 s3 ->
+  exists s3' M', Plus L3 s3 E0 s3' /\ (* idem *)
+           strong_equivalence2 M' s2' s3' /\
+           weak_equivalence1 M' s1 s3' /\
+      common_equivalence M' s1 s2' s3'.
+
+(* The weakly-related state takes a step, not the strongly-related states *)
+Hypothesis step_silent_weak1:
+  forall s1 s1', Step L1 s1 E0 s1' ->
+  forall s2 s3 M, strong_equivalence2 M s2 s3 ->
+           weak_equivalence1 M s1 s3 ->
+           common_equivalence M s1 s2 s3 ->
+  exists M', strong_equivalence2 M' s2 s3 /\
+        weak_equivalence1 M' s1' s3 /\
+        common_equivalence M' s1' s2 s3.
+        (* order (M', s1', s2) (M, s1, s2). *)
+
+Hypothesis step_silent_weak2:
+  forall s2 s2', Step L2 s2 E0 s2' ->
+  forall s1 s3 M, strong_equivalence1 M s1 s3 ->
+           weak_equivalence2 M s2 s3 ->
+           common_equivalence M s1 s2 s3 ->
+   exists M', strong_equivalence1 M' s1 s3 /\
+           weak_equivalence2 M' s2' s3 /\
+           common_equivalence M' s1 s2' s3.
+
+(* NOTE: should we add a lemma about internal steps that generate an event? *)
+
+(* The three states take a step at the same time, generating an event *)
+(* NOTE: is this lemma enough or should we enforce that the weak and strong relations
+   get swapped? -> i think no, but that's just an intuition that comes from the fact
+   we could imagine having two executions where private events are synchronized but
+   do not lead to a control swap *)
+Hypothesis step_event:
+  forall s1 e s1', Step L1 s1 (e :: nil) s1' ->
+  forall s2 s2',   Step L2 s2 (e :: nil) s2' ->
+  forall s3 M, match_states M s1 s2 s3    ->
+  exists s3' M', Plus L3 s3 (e :: nil) s3' /\ (* using Plus here because we know if an event is emitted then we've done at least one step *)
+            match_states M' s1' s2' s3'.
+
+Lemma threeway_simulation_diagram:
+  @threeway_simulation L1 L2 L3 single_L1 single_L2 single_L3.
+Proof.
+  eapply Threeway_simulation with
+    (match_states := fun s1 s2 s3 => exists M, match_states M s1 s2 s3).
+  econstructor; eauto.
+  - intros.
+    exploit match_initial_states; eauto.
+    intros [? [? [? ?]]]. eexists; split; eauto.
+  - intros s1 e s1' H s2 s2' H0 s3 [? ?].
+    exploit step_event; try now intuition eauto.
+    intros [? [? [? ?]]].
+    eexists; intuition eauto.
+  - intros ? ? step1 ? ? [M H].
+    inv H.
+    + exploit step_silent_strong1; eauto.
+      intros [? [? [? [? [? ?]]]]].
+      eexists; split; eauto using plus_star.
+      eexists; eauto using match_states_left.
+    + exploit step_silent_weak1; eauto.
+      intros [? [? [? ?]]].
+      eexists; split; eauto using star_refl.
+      eexists; eauto using match_states_right.
+  - intros ? ? step2 ? ? [M H].
+    inv H.
+    + exploit step_silent_weak2; eauto.
+      intros [? [? [? ?]]].
+      eexists; split; eauto using star_refl.
+      eexists; eauto using match_states_left.
+    + exploit step_silent_strong2; eauto.
+      intros [? [? [? [? [? ?]]]]].
+      eexists; split; eauto using plus_star.
+      eexists; eauto using match_states_right.
+Qed.
+
+End THREEWAY_SIMU_DIAGRAM.
